Switch to a relational interpretation for terms

theories/par.v
@@ -42,97 +42,37 @@ Inductive RTC  : Ty -> Ty -> Type :=
 Definition ICoherent A0 A1 : Type :=
   { B : Ty &  prod (RTC A0 B) (RTC A1 B)}.
 
-(* Based on https://poplmark-reloaded.github.io/coq/well-scoped/PR.sn_defs.html *)
-Inductive SN : Tm -> Prop :=
-| S_Neu a : SNe a -> SN a
-| S_Abs a : SN a -> SN (TmAbs a)
-| S_Red a0 a1 : SNRed a0 a1 -> SN a1 -> SN a0
-with SNe : Tm -> Prop :=
-| S_Var i : SNe (VarTm i)
-| S_App a b : SNe a -> SN b -> SNe (TmApp a b)
-with SNRed : Tm -> Tm -> Prop :=
-| S_AppL a0 a1 b :
-  SNRed a0 a1 ->
-  SNRed (TmApp a0 b) (TmApp a1 b)
-| S_AppAbs a b :
-  SN b ->
-  SNRed (TmApp (TmAbs a) b) (subst_Tm (b…) a).
+Inductive Red : Tm -> Tm -> Prop :=
+| R_App a0 a1 b :
+  Red a0 a1 ->
+  Red (TmApp a0 b) (TmApp a1 b)
+| R_AppAbs a b :
+  Red (TmApp (TmAbs b) a) (subst_Tm (a …) b).
 
-Scheme SN_ind_2 := Minimality for SN Sort Prop
-                   with SNe_ind_2 := Minimality for SNe Sort Prop
-                    with redSN_ind_2 := Minimality for SNRed Sort Prop.
-Combined Scheme SN_multind from SN_ind_2, SNe_ind_2, redSN_ind_2.
+Record CR (R : Tm -> Tm -> Prop) : Prop := CR_intro
+  { CR1a : forall a0 a1 b, Red a0 a1 -> R a1 b -> R a0 b
+  ; CR1b : forall a b0 b1, Red b0 b1 -> R a b1 -> R a b0
+  ; CR2 : forall a a' b b', R a a' -> R b b' -> R b a' -> R a b'}.
 
-Record CR (S : Tm -> Prop) : Prop := CR_intro
-  { CR1 : forall a, S a -> SN a
-  ; CR2 : forall a b, SNRed a b -> S b -> S a
-  ; CR3 : forall a, SNe a -> S a }.
+Lemma CR1 R : CR R -> forall a0 a1 b0 b1, Red a0 a1 -> Red b0 b1 -> R a1 b1 -> R a0 b0.
+Proof. hauto lq:on inv:CR. Qed.
 
-Hint Constructors CR SN SNRed SNe : rdb.
+Hint Constructors CR Red : rdb.
 
 Module red_props.
 
-  Lemma antirenaming :
-          (forall a, SN a -> forall ξ b, a = ren_Tm ξ b -> SN b) /\
-          (forall a, SNe a -> forall ξ b, a = ren_Tm ξ b -> SNe b) /\
-            (forall a b, SNRed a b -> forall ξ a', a = ren_Tm ξ a' -> exists b', b = ren_Tm ξ b' /\ SNRed a' b').
+  Lemma CR_Op R0 R1 : (forall a b, R0 a b <-> R1 b a) -> CR R0 -> CR R1.
+  Proof. hauto lq:on rew:off ctrs:CR inv:CR. Qed.
+
+  Lemma CR_Prod R0 R1 : CR R0 -> CR R1 ->
+         CR (fun b0 b1 => forall a0 a1, R0 a0 a1 -> R1 (TmApp b0 a0) (TmApp b1 a1)).
   Proof.
-    apply SN_multind.
-    - qauto use:S_Neu.
-    - move => a h ih ξ []//.
-      qauto use:S_Abs.
-    - qauto db:rdb.
-    - qauto use:S_Var inv:Tm.
-    - move => a b ha iha hb ihb ξ []//.
-      qauto db:rdb.
-    - move => a0 a1 b ha iha ξ []// a' b' [*]. subst.
-      specialize iha with (1 := eq_refl).
-      move : iha => [b0 [? ?]]. subst.
-      exists (TmApp b0 b'). split => //=.
-      by apply S_AppL.
-    - move => a b h ih ξ []// []// a' b' [*]. subst.
-      specialize ih with (1 := eq_refl).
-      exists (subst_Tm (b'…) a').
-      split. by asimpl.
-      by apply S_AppAbs.
+    hauto l:on ctrs:CR inv:CR.
   Qed.
 
-  Lemma ext (a : Tm) i :
-    SN (TmApp a (VarTm i)) ->
-    SN a.
+  Lemma CR_Forall {A} (x : A) (P : A -> Prop) (_ : P x) F : (forall a : A, P a -> CR (F a)) -> CR (fun b0 b1 => forall a, P a -> F a b0 b1).
   Proof.
-    move E : (TmApp a (VarTm i)) => v h.
-    move : i a E.
-    elim : v /h => //=.
-    - hauto lq:on inv:SNe use:S_Neu.
-    - move => a0 a1 ha0 ha1 ih.
-      move => i a ?. subst.
-      inversion ha0; subst.
-      hauto lq:on inv:SN, SNe ctrs:SN.
-      apply S_Abs.
-      move : ha1.
-      have -> : subst_Tm (VarTm i…) a0 = ren_Tm (i…) a0 by substify; asimpl.
-      qauto use:antirenaming.
-  Qed.
-
-  Lemma CR_Prod s0 s1 : CR s0 -> CR s1 -> CR (fun b => forall a, s0 a -> s1 (TmApp b a)).
-  Proof.
-    move=>*.
-    apply CR_intro.
-    - hauto q:on use:CR1, CR3, S_Var, ext.
-    - hauto lq:on ctrs:SNRed inv:CR.
-    - hauto lq:on ctrs:SNe inv:CR.
-  Qed.
-
-  Lemma CR_SN : CR SN.
-  Proof.
-    apply CR_intro; eauto with rdb.
-  Qed.
-
-  Lemma CR_Forall {A} (x : A) (P : A -> Prop) (_ : P x) F : (forall a : A, P a -> CR (F a)) -> CR (fun b => forall a, P a -> F a b).
-  Proof.
-    move => hF.
-    apply CR_intro; firstorder.
+    hauto q:on ctrs:CR inv:CR.
   Qed.
 
 End red_props.
